.

cfrontend/BeePL.v
@@ -346,32 +346,102 @@ Section Big_step_semantics.
 Variable ge : genv.
 
 (* Would be useful in proving equivalence with Cstrategy for simpl expressions *)
-Inductive bsem_expr : vmap -> mem -> expr -> mem -> value -> Prop :=
-| bsem_val : forall vm hm v t,
-             bsem_expr vm hm (Val v t) hm v
-| bsem_var : forall vm hm x v t l, 
-             vm!(x.(vname)) = Some (l, t) ->
-             t = x.(vtype) ->
-             deref_addr t hm l Ptrofs.zero Full v ->
-             bsem_expr vm hm (Var x) hm v
-| bsem_gvar : forall vm hm x v t l, 
+Inductive bsem_expr_slv : vmap -> mem -> expr -> positive -> ptrofs -> bitfield -> Prop :=
+| bsem_var : forall vm hm x t l, 
+              vm!(x.(vname)) = Some (l, t) ->
+              t = x.(vtype) ->
+              bsem_expr_slv vm hm (Var x) l Ptrofs.zero Full
+| bsem_gvar : forall vm hm x t l, 
               vm!(x.(vname)) = None ->
               Genv.find_symbol ge x.(vname) = Some l ->
               t = x.(vtype) ->
-              deref_addr t hm l Ptrofs.zero Full v ->
-              bsem_expr vm hm (Var x) hm v
+              bsem_expr_slv vm hm (Var x) l Ptrofs.zero Full
+| bsem_addr : forall vm hm l ofs,
+              bsem_expr_slv vm hm (Addr l ofs) l.(lname) ofs l.(lbitfield)
+| bsem_prim_deref : forall vm hm hm' e t l ofs, 
+                    bsem_expr_srv vm hm e hm' (Vloc l ofs) ->
+                    bsem_expr_slv vm hm' (Prim Deref (e :: nil) t) l ofs Full
+with bsem_expr_srv : vmap -> mem -> expr -> mem -> value -> Prop :=
+| bsem_val : forall vm hm v t,
+             bsem_expr_srv vm hm (Val v t) hm v
 | bsem_const_int : forall vm hm i t, 
-                   bsem_expr vm hm (Const (ConsInt i) t) hm (Vint i)
+                   bsem_expr_srv vm hm (Const (ConsInt i) t) hm (Vint i)
 | bsem_const_int64 : forall vm hm i t, 
-                     bsem_expr vm hm (Const (ConsLong i) t) hm (Vint64 i)
-| bsem_const_unit : forall vm hm,
-                    bsem_expr vm hm (Const (ConsUnit) (Ptype Tunit)) hm (Vunit)
+                     bsem_expr_srv vm hm (Const (ConsLong i) t) hm (Vint64 i)
+| bsem_const_uint : forall vm hm, 
+                    bsem_expr_srv vm hm (Const (ConsUnit) (Ptype Tunit)) hm (Vunit)
+| bsem_loc_rv : forall hm vm t l ofs v,
+                bsem_expr_slv vm hm (Addr l ofs) l.(lname) ofs l.(lbitfield) ->
+                t = l.(ltype) ->
+                deref_addr t hm l.(lname) ofs Full v ->
+                bsem_expr_srv vm hm (Addr l ofs) hm v
+| bsem_prim_ref : forall vm hm e v t hm' hm'' l, 
+                  bsem_expr_srv vm hm e hm' v ->
+                  Mem.alloc hm 0 (sizeof_type (typeof_expr e)) = (hm', l) ->
+                  assign_addr (typeof_expr e) hm' l Ptrofs.zero Full v hm'' v ->
+                  bsem_expr_srv vm hm (Prim Ref (e :: nil) t) hm'' (Vloc l Ptrofs.zero)
+| bsem_prim_uop : forall vm hm e v uop  v' t ct v'',
+                  bsem_expr_srv vm hm e hm v ->
+                  transBeePL_type (typeof_expr e) = OK ct ->
+                  sem_unary_operation uop (transBeePL_value_cvalue v) ct hm = Some v' ->
+                  transC_val_bplvalue v' = OK v'' ->
+                  bsem_expr_srv vm hm (Prim (Uop uop) (e :: nil) t) hm v''
+| bsem_prim_bop : forall vm hm cenv e1 e2 t v1 v2 bop v ct1 ct2 v',
+                  bsem_expr_srv vm hm e1 hm v1 ->
+                  bsem_expr_srv vm hm e2 hm v2 ->
+                  transBeePL_type (typeof_expr e1) = OK ct1 ->
+                  transBeePL_type (typeof_expr e2) = OK ct2 ->
+                  sem_binary_operation cenv bop (transBeePL_value_cvalue v1) ct1 (transBeePL_value_cvalue v2) ct2 hm = Some v ->
+                  transC_val_bplvalue v = OK v' ->
+                  bsem_expr_srv vm hm (Prim (Bop bop) (e1 :: e2 :: nil) t) hm v'
+| bsem_unit : forall vm hm, 
+              bsem_expr_srv vm hm (Unit (Ptype Tunit)) hm Vunit.
+
+Scheme bsem_expr_slv_mut := Minimality for bsem_expr_slv Sort Prop
+  with bsem_expr_srv_mut := Minimality for bsem_expr_srv Sort Prop.
+Combined Scheme bsem_expr_slv_srv_mut from bsem_expr_slv_mut,bsem_expr_srv_mut.
+
+Inductive bsem_expr_srvs : vmap -> mem -> list expr -> mem -> list value -> Prop :=
+| bsem_expr_srv_nil : forall vm hm, 
+                      bsem_expr_srvs vm hm nil hm nil
+| bsem_expr_srv_cons : forall vm hm e es v vs hm' hm'',
+                       bsem_expr_srv vm hm e hm' v ->
+                       bsem_expr_srvs vm hm' es hm'' vs ->
+                       bsem_expr_srvs vm hm (e :: es) hm'' (v :: vs).
+
+
+Inductive bsem_expr : vmap -> mem -> expr -> mem -> value -> Prop :=
+| bsem_prim_massgn : forall vm hm e1 e2 l ofs v hm' hm'' hm''' ct1 ct2 bf v', (* Fix me *)
+                     bsem_expr_slv vm hm e1 l ofs bf -> 
+                     bsem_expr_srv vm hm e2 hm' v ->
+                     transBeePL_type (typeof_expr e1) = OK ct1 ->
+                     transBeePL_type (typeof_expr e2) = OK ct2 ->
+                     sem_cast (transBeePL_value_cvalue v) ct2 ct1 hm'' = Some (transBeePL_value_cvalue v') ->
+                     assign_addr (typeof_expr e1) hm'' l ofs bf v' hm''' v' ->
+                     bsem_expr vm hm (Prim Massgn (e1 :: e2 :: nil) (typeof_expr e1)) hm''' Vunit
+| bsem_bind : forall vm hm x t e e' t' hm1 v e'' v' hm2 hm3,
+              bsem_expr_srv vm hm e hm1 v ->
+              subst vm hm1 x v e' hm2 e'' ->
+              bsem_expr vm hm2 e'' hm3 v' ->
+              bsem_expr vm hm (Bind x t e e' t') hm3 v'
+| bsem_cond_true : forall vm hm e1 hm' e2 hm'' e3 t vb v ct1, 
+                   bsem_expr_srv vm hm e1 hm' vb -> 
+                   transBeePL_type (typeof_expr e1) = OK ct1 ->
+                   bool_val (transBeePL_value_cvalue vb) ct1 hm = Some true ->
+                   bsem_expr vm hm' e2 hm'' v ->
+                   bsem_expr vm hm (Cond e1 e2 e3 t) hm'' v
+| bsem_cond_false : forall vm hm e1 hm' e2 hm'' e3 t vb v ct1, 
+                    bsem_expr_srv vm hm e1 hm' vb -> 
+                    transBeePL_type (typeof_expr e1) = OK ct1 ->
+                    bool_val (transBeePL_value_cvalue vb) ct1 hm = Some false ->
+                    bsem_expr vm hm' e3 hm'' v ->
+                    bsem_expr vm hm (Cond e1 e2 e3 t) hm'' v
 | bsem_appr : forall vm1 hm1 e es t l fd hm2 hm3 hm4 hm5 hm6 vm2 vs rv r hm7,
-              bsem_expr vm1 hm1 e hm2 (Vloc l Ptrofs.zero) ->
+              bsem_expr_srv vm1 hm1 e hm2 (Vloc l Ptrofs.zero) ->
               Genv.find_funct ge (transBeePL_value_cvalue (Vloc l Ptrofs.zero)) = Some (Internal fd) ->
               list_norepet (fd.(fn_args) ++ fd.(fn_vars)) ->
               alloc_variables vm1 hm2 (fd.(fn_args) ++ fd.(fn_vars)) vm2 hm3 -> 
-              bsem_exprs vm2 hm3 es hm4 vs ->
+              bsem_expr_srvs vm2 hm3 es hm4 vs ->
               typeof_values vs (extract_types_vinfos fd.(fn_args)) ->
               bind_variables vm1 hm4 fd.(fn_args) vs hm5  ->
               bsem_expr vm1 hm5 fd.(fn_body) hm6 rv -> 
@@ -383,71 +453,13 @@ Inductive bsem_expr : vmap -> mem -> expr -> mem -> value -> Prop :=
              Genv.find_funct ge (transBeePL_value_cvalue (Vloc l Ptrofs.zero)) = Some (Internal fd) ->
              list_norepet (fd.(fn_args) ++ fd.(fn_vars)) ->
              alloc_variables vm1 hm2 (fd.(fn_args) ++ fd.(fn_vars)) vm2 hm3 -> 
-             bsem_exprs vm2 hm3 es hm4 vs ->
+             bsem_expr_srvs vm2 hm3 es hm4 vs ->
              typeof_values vs (extract_types_vinfos fd.(fn_args)) ->
              bind_variables vm1 hm4 fd.(fn_args) vs hm5  ->
              bsem_expr vm1 hm5 fd.(fn_body) hm6 rv -> 
              typeof_value rv (fd.(fn_return)) ->
-             bsem_expr vm1 hm1 (App None e es t) hm6 rv 
-| bsem_prim_uop : forall vm hm e v uop  v' t ct v'',
-                  bsem_expr vm hm e hm v ->
-                  transBeePL_type (typeof_expr e) = OK ct ->
-                  sem_unary_operation uop (transBeePL_value_cvalue v) ct hm = Some v' ->
-                  transC_val_bplvalue v' = OK v'' ->
-                  bsem_expr vm hm (Prim (Uop uop) (e :: nil) t) hm v''
-| bsem_prim_bop : forall vm hm cenv e1 e2 t v1 v2 bop v ct1 ct2 v',
-                  bsem_expr vm hm e1 hm v1 ->
-                  bsem_expr vm hm e2 hm v2 ->
-                  transBeePL_type (typeof_expr e1) = OK ct1 ->
-                  transBeePL_type (typeof_expr e2) = OK ct2 ->
-                  sem_binary_operation cenv bop (transBeePL_value_cvalue v1) ct1 (transBeePL_value_cvalue v2) ct2 hm = Some v ->
-                  transC_val_bplvalue v = OK v' ->
-                  bsem_expr vm hm (Prim (Bop bop) (e1 :: e2 :: nil) t) hm v'
-| bsem_prim_ref : forall vm hm e t ct hm' v l, 
-                  bsem_expr vm hm e hm' v ->
-                  transBeePL_type (typeof_expr e) = OK ct ->
-                  Mem.alloc hm 0 (sizeof_type t) = (hm', l) ->
-                  bsem_expr vm hm (Prim Ref (e :: nil) t) hm' (Vloc l Ptrofs.zero)
-| bsem_prim_deref : forall vm hm e t l ofs hm' v, 
-                    bsem_expr vm hm e hm' (Vloc l ofs) ->
-                    deref_addr t hm l ofs Full v ->
-                    bsem_expr vm hm (Prim Deref (e :: nil) t) hm' v
-| bsem_prim_massgn : forall vm hm e1 e2 l ofs v hm' hm'' hm''' ct1 ct2 bf v', (* Fix me *)
-                     bsem_expr vm hm e1 hm' (Vloc l ofs) -> 
-                     bsem_expr vm hm' e2 hm'' v ->
-                     transBeePL_type (typeof_expr e1) = OK ct1 ->
-                     transBeePL_type (typeof_expr e2) = OK ct2 ->
-                     sem_cast (transBeePL_value_cvalue v) ct2 ct1 hm'' = Some (transBeePL_value_cvalue v') ->
-                     assign_addr (typeof_expr e1) hm'' l ofs bf v' hm''' v' ->
-                     bsem_expr vm hm (Prim Massgn (e1 :: e2 :: nil) (typeof_expr e1)) hm''' Vunit
-| bsem_bind : forall vm hm x t e e' t' hm1 v e'' v' hm2 hm3,
-              bsem_expr vm hm e hm1 v ->
-              subst vm hm1 x v e' hm2 e'' ->
-              bsem_expr vm hm2 e'' hm3 v' ->
-              bsem_expr vm hm (Bind x t e e' t') hm3 v'
-| bsem_cond_true : forall vm hm e1 hm' e2 hm'' e3 t vb v ct1, 
-                   bsem_expr vm hm e1 hm' vb -> 
-                   transBeePL_type (typeof_expr e1) = OK ct1 ->
-                   bool_val (transBeePL_value_cvalue vb) ct1 hm = Some true ->
-                   bsem_expr vm hm' e2 hm'' v ->
-                   bsem_expr vm hm (Cond e1 e2 e3 t) hm'' v
-| bsem_cond_false : forall vm hm e1 hm' e2 hm'' e3 t vb v ct1, 
-                    bsem_expr vm hm e1 hm' vb -> 
-                    transBeePL_type (typeof_expr e1) = OK ct1 ->
-                    bool_val (transBeePL_value_cvalue vb) ct1 hm = Some false ->
-                    bsem_expr vm hm' e3 hm'' v ->
-                    bsem_expr vm hm (Cond e1 e2 e3 t) hm'' v
-| bsem_unit : forall vm hm, 
-              bsem_expr vm hm (Unit (Ptype Tunit)) hm Vunit
-| bsem_addr : forall vm hm l ofs,
-              bsem_expr vm hm (Addr l ofs) hm (Vloc l.(lname) ofs)
-with bsem_exprs : vmap -> mem -> list expr -> mem -> list value -> Prop :=
-| bsem_nil : forall vm hm,
-             bsem_exprs vm hm nil hm nil
-| bsem_cons : forall vm hm hm' hm'' v vs e es,
-              bsem_expr vm hm e hm' v ->
-              bsem_exprs vm hm' es hm'' vs ->
-              bsem_exprs vm hm' (e :: es) hm'' (v :: vs).
+             bsem_expr vm1 hm1 (App None e es t) hm6 rv.              
+               
 
 End Big_step_semantics.
 
@@ -463,18 +475,19 @@ Inductive sem_expr : vmap -> mem -> expr -> mem -> expr -> Prop :=
                  sem_expr vm hm (Val (Vint i) t) hm (Val (Vint i) t)
 | sem_val_int64 : forall vm hm i t,
                   sem_expr vm hm (Val (Vint64 i) t) hm (Val (Vint64 i) t)
-| sem_val_loc : forall vm hm t v l ofs,
-                deref_addr t hm l ofs Full v ->
-                sem_expr vm hm (Val (Vloc l ofs) t) hm (Val v t)
+| sem_val_loc : forall vm hm t l ofs,
+                sem_expr vm hm (Val (Vloc l ofs) t) hm (Val (Vloc l ofs) t)
 | sem_var : forall vm hm x t l,
             vm!(x.(vname)) = Some (l, t) ->
             t = x.(vtype) ->
-            sem_expr vm hm (Var x) hm (Val (Vloc l Ptrofs.zero) t)
+            sem_expr vm hm (Var x) hm 
+            (Addr {| lname := l; ltype := t; lbitfield := Full |} Ptrofs.zero)
 | sem_gvar : forall vm hm x t l,
              vm!(x.(vname)) = None ->
              t = x.(vtype) ->
              Genv.find_symbol ge x.(vname) = Some l ->
-             sem_expr vm hm (Var x) hm (Val (Vloc l Ptrofs.zero) t)
+             sem_expr vm hm (Var x) hm 
+             (Addr {| lname := l; ltype := t; lbitfield := Full |} Ptrofs.zero)
 | sem_const_int : forall vm hm i t, 
                   sem_expr vm hm (Const (ConsInt i) t) hm (Val (Vint i) t)
 | sem_const_int64 : forall vm hm i t, 
@@ -504,10 +517,11 @@ Inductive sem_expr : vmap -> mem -> expr -> mem -> expr -> Prop :=
 | sem_prim_ref : forall vm hm e e' t hm',
                  sem_expr vm hm e hm' e' ->
                  sem_expr vm hm (Prim Ref (e :: nil) t) hm' (Prim Ref (e' :: nil) t)
-| sem_prim_refv : forall vm hm v tv t ct hm' l,
+| sem_prim_refv : forall vm hm v tv t ct hm' hm'' l,
                   transBeePL_type tv = OK ct ->
                   Mem.alloc hm 0 (sizeof_type t) = (hm', l) ->
-                  sem_expr vm hm (Prim Ref ((Val v tv) :: nil) t) hm' (Val (Vloc l Ptrofs.zero) t)
+                  assign_addr tv hm' l Ptrofs.zero Full v hm'' v ->
+                  sem_expr vm hm (Prim Ref ((Val v tv) :: nil) t) hm'' (Val (Vloc l Ptrofs.zero) t)
 | sem_prim_deref : forall vm hm e t hm' e',
                    sem_expr vm hm e hm' e' ->
                    sem_expr vm hm (Prim Deref (e :: nil) t) hm' (Prim Deref (e' :: nil) t)
@@ -552,14 +566,13 @@ Inductive sem_expr : vmap -> mem -> expr -> mem -> expr -> Prop :=
               Genv.find_funct ge (transBeePL_value_cvalue v) = Some (Internal fd) ->
               list_norepet (fd.(fn_args) ++ fd.(fn_vars)) ->
               alloc_variables vm hm (fd.(fn_args) ++ fd.(fn_vars)) vm1 hm1 -> 
-              bsem_exprs ge vm1 hm1 es hm2 vs ->
+              bsem_expr_srvs ge vm1 hm1 es hm2 vs ->
               typeof_values vs (extract_types_vinfos fd.(fn_args)) ->
               bind_variables vm1 hm2 fd.(fn_args) vs hm3  ->
               bsem_expr ge vm1 hm3 fd.(fn_body) hm4 rv ->
               bind_variables vm1 hm4 (r::nil) (rv::nil) hm5 ->
               typeof_value rv (fd.(fn_return)) ->
               sem_expr vm hm (App (Some r.(vname)) (Val v (Ftype ts ef rt)) es t) hm5 (Val rv fd.(fn_return))
-(* Fix me *)
 | sem_addr : forall vm hm t l bf ofs v,
              deref_addr t hm l ofs bf v ->
              sem_expr vm hm (Addr {| lname := l; ltype := t; lbitfield := bf |} ofs) hm (Val v t).
